refactor memory module
parametrise memory by its type of elements

Memory.v
@@ -4,61 +4,61 @@ Require Import ZArith.
 
 Definition adr := nat.
 
-Definition Mem : Set := adr -> nat.
+Definition Mem (T : Type) : Type := adr -> T.
 
-Definition get (r : adr) (m : Mem) : nat := m r.
+Definition get {T} (r : adr) (m : Mem T) : T := m r.
 
-Definition set (r : adr) (v : nat) (m : Mem) : Mem :=
+Definition set {T} (r : adr) (v : T) (m : Mem T) : Mem T :=
   fun r' => if eqb r r' then v else get r' m.
 
-Definition Eqr (r : adr) (m1 m2 : Mem) :=
+Definition Eqr {T} (r : adr) (m1 m2 : Mem T) :=
   forall i : adr, i < r -> get i m1 = get i m2.
 
 Notation "x =[ r ] y" := (Eqr r x y) (at level 70).
 
 
-Lemma eqr_refl x r : x =[ r ] x.
+Lemma eqr_refl T (x : Mem T) r : x =[ r ] x.
 Proof. intros i H. reflexivity. Qed.
 
-Lemma eqr_sym x y r : x =[ r ] y -> y =[ r ] x.
+Lemma eqr_sym T (x y : Mem T) r : x =[ r ] y -> y =[ r ] x.
 Proof. intros R i E. apply R in E. auto. Qed.
 
-Lemma eqr_trans x y z r : x =[ r ] y -> y =[ r ] z -> x =[ r ] z.
+Lemma eqr_trans T (x y z : Mem T) r : x =[ r ] y -> y =[ r ] z -> x =[ r ] z.
 Proof.
   unfold Eqr. intros H1 H2 i R. pose (H1 i R) as E1. pose (H2 i R) as E2.
   rewrite E1. auto.
 Qed. 
 
-Lemma eqr_less x y r r' : x =[ r ] y -> r' <= r -> x =[ r' ] y.
+Lemma eqr_less T (x y : Mem T) r r' : x =[ r ] y -> r' <= r -> x =[ r' ] y.
 Proof. intros R L i L'. apply R. omega. Qed.
 
 
-Lemma set_get_neq r i s n : r <> i -> get i s = get i (set r n s).
+Lemma set_get_neq T r i (s : Mem T) n : r <> i -> get i s = get i (set r n s).
 Proof.
   intro E. unfold get, set. remember (r =? i) as t. destruct t.
   - rewrite <- Nat.eqb_neq in *. rewrite E in *. inversion Heqt.
   - reflexivity.
 Qed.
 
-Lemma set_eqr n s s' r r' : set r n s =[r'] s' -> r < r' -> s =[r] s'.
+Lemma set_eqr T n (s s' : Mem T) r r' : set r n s =[r'] s' -> r < r' -> s =[r] s'.
 Proof.
   intros H R i E. assert (i < r') as E' by omega. apply H in E'. rewrite <- E'.
   apply set_get_neq. omega.
 Qed.
 
 
-Lemma set_get r s n : get r (set r n s) = n.
+Lemma set_get T r (s : Mem T) n : get r (set r n s) = n.
 Proof.
   unfold get, set. rewrite <- beq_nat_refl. reflexivity.
 Qed.
 
-Lemma set_get_eqr r r' s s' n : set r n s =[r'] s' -> r < r' -> get r s' = n.
+Lemma set_get_eqr T r r' (s s' : Mem T) n : set r n s =[r'] s' -> r < r' -> get r s' = n.
 Proof.
   intros R E. apply R in E. rewrite <- E. apply set_get.
 Qed.
 
 
-Lemma set_eqr_incr r s s' n : s =[r] s' -> set r n s =[r + 1] set r n s'.
+Lemma set_eqr_incr T r (s s' : Mem T) n : s =[r] s' -> set r n s =[r + 1] set r n s'.
 Proof.
   admit.
 Admitted.
